-

RingLike.v
@@ -124,7 +124,7 @@ Notation "- 1" := (rngl_opp rngl_one) : ring_like_scope.
 
 Inductive not_applicable := NA.
 
-Definition zero_dividor {T} {ro : ring_like_op T} a :=
+Definition is_zero_divisor {T} {ro : ring_like_op T} a :=
   ∃ b, b ≠ 0%F ∧ (a * b = 0)%F.
 
 Fixpoint rngl_of_nat {T} {ro : ring_like_op T} n :=
@@ -178,19 +178,19 @@ Class ring_like_prop T {ro : ring_like_op T} :=
       else not_applicable;
     (* when has inverse *)
     rngl_opt_mul_inv_l :
-      if rngl_has_inv then ∀ a : T, not (zero_dividor a) → (¹/ a * a = 1)%F
+      if rngl_has_inv then ∀ a : T, not (is_zero_divisor a) → (¹/ a * a = 1)%F
       else not_applicable;
     rngl_opt_mul_inv_r :
       if (rngl_has_inv && negb rngl_is_comm)%bool then
-        ∀ a : T, ¬ zero_dividor a → (a / a = 1)%F
+        ∀ a : T, ¬ is_zero_divisor a → (a / a = 1)%F
       else not_applicable;
     (* when has division (quot) *)
     rngl_opt_mul_quot_l :
-      if rngl_has_quot then ∀ a b, ¬ zero_dividor a → (a * b / a)%F = b
+      if rngl_has_quot then ∀ a b, ¬ is_zero_divisor a → (a * b / a)%F = b
       else not_applicable;
     rngl_opt_mul_quot_r :
       if (rngl_has_quot && negb rngl_is_comm)%bool then
-        ∀ a b, ¬ zero_dividor b → (a * b / b)%F = a
+        ∀ a b, ¬ is_zero_divisor b → (a * b / b)%F = a
       else not_applicable;
     (* when equality is decidable *)
     rngl_opt_eq_dec :
@@ -200,10 +200,10 @@ Class ring_like_prop T {ro : ring_like_op T} :=
     rngl_opt_le_dec :
       if rngl_has_dec_le then ∀ a b : T, ({a ≤ b} + {¬ a ≤ b})%F
       else not_applicable;
-    (* when has_no_zero_divisors *)
+    (* when has_no_is_zero_divisors *)
     rngl_opt_integral :
       if rngl_is_integral then
-        ∀ a b, (a * b = 0)%F → zero_dividor a ∨ b = 0%F
+        ∀ a b, (a * b = 0)%F → is_zero_divisor a ∨ b = 0%F
       else not_applicable;
     (* characteristic *)
     rngl_characteristic_prop :
@@ -320,7 +320,7 @@ Qed.
 
 Theorem rngl_mul_inv_l :
   rngl_has_inv = true →
-  ∀ a : T, ¬ zero_dividor a → (¹/ a * a = 1)%F.
+  ∀ a : T, ¬ is_zero_divisor a → (¹/ a * a = 1)%F.
 Proof.
 intros H1 *.
 specialize rngl_opt_mul_inv_l as H.
@@ -640,7 +640,7 @@ Qed.
 
 Theorem rngl_mul_inv_r :
   rngl_has_inv = true ∨ rngl_has_quot = true →
-  ∀ a : T, ¬ zero_dividor a → (a / a = 1)%F.
+  ∀ a : T, ¬ is_zero_divisor a → (a / a = 1)%F.
 Proof.
 intros Hii * Haz.
 remember rngl_has_inv as iv eqn:Hiv; symmetry in Hiv.
@@ -669,7 +669,7 @@ Qed.
 
 Theorem rngl_mul_div_l :
   rngl_has_inv = true ∨ rngl_has_quot = true →
-  ∀ a b : T, ¬ zero_dividor b → (a * b / b)%F = a.
+  ∀ a b : T, ¬ is_zero_divisor b → (a * b / b)%F = a.
 Proof.
 intros Hii a b Hbz.
 remember rngl_has_inv as iv eqn:Hiv; symmetry in Hiv.
@@ -699,7 +699,7 @@ Qed.
 Theorem rngl_div_0_l :
   (rngl_has_opp = true ∨ rngl_has_sous = true) ∧
   (rngl_has_inv = true ∨ rngl_has_quot = true) →
-  ∀ a, ¬ zero_dividor a → (0 / a)%F = 0%F.
+  ∀ a, ¬ is_zero_divisor a → (0 / a)%F = 0%F.
 Proof.
 intros Hiv * Haz.
 remember (0 / a)%F as x eqn:Hx.
@@ -714,7 +714,7 @@ Theorem rngl_integral :
   rngl_has_opp = true ∨ rngl_has_sous = true →
   (rngl_is_integral ||
    ((rngl_has_inv || rngl_has_quot) && rngl_has_dec_eq))%bool = true →
-  ∀ a b, (a * b = 0)%F → zero_dividor a ∨ b = 0%F.
+  ∀ a b, (a * b = 0)%F → is_zero_divisor a ∨ b = 0%F.
 Proof.
 intros Hmo Hdo * Hab.
 specialize rngl_opt_integral as rngl_integral.
@@ -731,17 +731,17 @@ destruct iv. {
   rewrite rngl_mul_0_r in H; [ | easy ].
 (**)
 ...
-zero_dividor must be decidable
+is_zero_divisor must be decidable
 ...
   destruct (rngl_eq_dec Hde a 0%F) as [Haz| Haz]. {
     left; subst a.
-    unfold zero_dividor.
+    unfold is_zero_divisor.
     exists 1%F.
     rewrite rngl_mul_0_l; [ | easy ].
     split; [ | easy ].
 ...
     intros H1.
-    unfold not_zero_dividor in H1.
+    unfold not_is_zero_divisor in H1.
     cbn in H1.
     apply H1 with (b := 1%F); [ | now apply rngl_mul_0_l ].
     apply rngl_1_neq_0.
